theories/typing/function.v
@@ -10,8 +10,8 @@ Section fn.
   Record fn_params := FP { fp_E : lft → elctx; fp_tys : vec type n; fp_ty : type }.
 
   Definition FP_wf E (tys : vec type n) `{!TyWfLst tys} ty `{!TyWf ty} :=
-    FP (λ ϝ, E ϝ ++ tys.(tyl_wf_E) ++ tys.(tyl_outlives_E) ϝ ++
-                    ty.(ty_wf_E) ++ ty.(ty_outlives_E) ϝ)
+    FP (λ ϝ, E ϝ ++ tyl_wf_E tys ++ tyl_outlives_E tys ϝ ++
+                    ty.(ty_wf_E) ++ ty_outlives_E ty ϝ)
        tys ty.
 
   (* The other alternative for defining the fn type would be to state
