theories/typing/uniq_bor.v
@@ -42,7 +42,7 @@ Section uniq_bor.
   Qed.
 
   Global Instance uniq_bor_wf κ ty `{!TyWf ty} : TyWf (uniq_bor κ ty) :=
-    { ty_lfts := [κ]; ty_wf_E := ty.(ty_wf_E) ++ ty.(ty_outlives_E) κ }.
+    { ty_lfts := [κ]; ty_wf_E := ty.(ty_wf_E) ++ ty_outlives_E ty κ }.
 
   Global Instance uniq_mono E L :
     Proper (flip (lctx_lft_incl E L) ==> eqtype E L ==> subtype E L) uniq_bor.
